NuStd_Base.thy
@@ -1,10 +1,652 @@
 theory NuStd_Base
-  imports  NuInstructions
+  imports NuSys NuBasicAbstractors NuInstructions
+  keywords
+     "\<up>:" "\<Up>:" "\<down>:" "\<Down>:" "subj" "always" "heap" "--" :: quasi_command
+  abbrevs "|^" = "\<up>"
+    and "||^" = "\<Up>"
+    and "|v" = "\<down>"
+    and "||v" = "\<Down>"
+    and "<up>" = "\<up>"
+    and "<down>" = "\<down>"
+    and "<Up>" = "\<Up>"
+    and "<Down>" = "\<Down>"
 begin
 
-\<nu>overloads split pop
+\<nu>overloads split and pop and merge
 
 declare Separation_assoc[simp]
+
+declare Nat.One_nat_def[simp del] Num.add_2_eq_Suc'[simp del] split_paired_All[simp del]
+declare Separation_assoc[simp]
+
+section \<open>Structural instructions\<close>
+
+subsection \<open>Basic sequential instructions\<close>
+
+subsubsection \<open>crash\<close>
+
+lemma crash_\<nu>app[no_atp]:  "\<^bold>p\<^bold>r\<^bold>o\<^bold>c op_crash \<blangle> X \<longmapsto> Y \<brangle>" unfolding \<nu>def op_crash_def by auto
+
+subsubsection \<open>drop\<close>
+
+declare op_drop_def[\<nu>instr]
+theorem drop_\<nu>app: "\<^bold>p\<^bold>r\<^bold>o\<^bold>c op_drop \<blangle> R\<heavy_comma> X\<heavy_comma> \<^bold>h\<^bold>e\<^bold>a\<^bold>p Nothing \<longmapsto> R\<heavy_comma> \<^bold>h\<^bold>e\<^bold>a\<^bold>p Nothing \<brangle>"
+  unfolding \<nu>def op_drop_def by (auto simp add: nu_exps)
+
+subsubsection \<open>duplication\<close>
+
+declare op_dup_def[\<nu>instr]
+theorem dup_\<nu>app: "\<^bold>p\<^bold>r\<^bold>o\<^bold>c op_dup \<blangle> R\<heavy_comma> X\<heavy_comma> \<^bold>h\<^bold>e\<^bold>a\<^bold>p Nothing \<longmapsto> R\<heavy_comma> X\<heavy_comma> X\<heavy_comma> \<^bold>h\<^bold>e\<^bold>a\<^bold>p Nothing\<brangle>"
+  unfolding \<nu>def op_dup_def by (auto simp add: nu_exps)
+
+
+subsubsection \<open>pair & de-pair\<close>
+
+(* declare op_pair_def[\<nu>instr] op_depair_def[\<nu>instr] *)
+
+lemma pr_\<nu>app: "\<^bold>p\<^bold>r\<^bold>o\<^bold>c op_pair \<blangle> R \<heavy_comma> a \<tycolon> A \<heavy_comma> b \<tycolon> B\<heavy_comma> \<^bold>h\<^bold>e\<^bold>a\<^bold>p Nothing \<longmapsto> R \<heavy_comma> (a,b) \<tycolon> (A \<cross_product> B)\<heavy_comma> \<^bold>h\<^bold>e\<^bold>a\<^bold>p Nothing \<brangle>"
+  unfolding \<nu>def  op_pair_def by (auto simp add: nu_exps)
+lemma dpr_\<nu>app: "\<^bold>p\<^bold>r\<^bold>o\<^bold>c op_depair \<blangle> R \<heavy_comma> (a,b) \<tycolon> (A \<cross_product> B)\<heavy_comma> \<^bold>h\<^bold>e\<^bold>a\<^bold>p Nothing \<longmapsto> R \<heavy_comma> a \<tycolon> A \<heavy_comma> b \<tycolon> B\<heavy_comma> \<^bold>h\<^bold>e\<^bold>a\<^bold>p Nothing \<brangle>"
+  unfolding \<nu>def  op_depair_def by (auto simp add: nu_exps)
+
+lemma hpr_\<nu>app: "\<^bold>c\<^bold>a\<^bold>s\<^bold>t H \<heavy_asterisk> h1 \<tycolon> H1 \<heavy_asterisk> h2 \<tycolon> H2 \<longmapsto> H \<heavy_asterisk> (h2,h1) \<tycolon> H2 \<^emph> H1"
+  unfolding Cast_def SepNu_to_SepSet Separation_assoc by blast
+lemma hdpr_\<nu>app: "\<^bold>c\<^bold>a\<^bold>s\<^bold>t H \<heavy_asterisk> (h2,h1) \<tycolon> H2 \<^emph> H1 \<longmapsto> H \<heavy_asterisk> h1 \<tycolon> H1 \<heavy_asterisk> h2 \<tycolon> H2"
+  unfolding Cast_def SepNu_to_SepSet Separation_assoc by blast
+
+(* \<nu>processor pair_auto_dest 30 \<open>\<^bold>c\<^bold>u\<^bold>r\<^bold>r\<^bold>e\<^bold>n\<^bold>t blk \<^bold>r\<^bold>e\<^bold>s\<^bold>u\<^bold>l\<^bold>t\<^bold>s \<^bold>i\<^bold>n (R\<heavy_comma> (a,b) \<tycolon> (A \<nuFusion>' B) \<flower> W)\<close> \<open>fn ctx => fn meta => Scan.succeed (fn _ =>
+  meta |> NuBasics.apply_proc_naive @{thm dpr_auto_schema} |> NuSys.accept_proc ctx)\<close>
+\<nu>processor pair_auto_dest' 30 \<open>\<^bold>c\<^bold>u\<^bold>r\<^bold>r\<^bold>e\<^bold>n\<^bold>t blk \<^bold>r\<^bold>e\<^bold>s\<^bold>u\<^bold>l\<^bold>t\<^bold>s \<^bold>i\<^bold>n (R\<heavy_comma> (a,b) \<tycolon> (A \<nuFusion>' B))\<close> \<open>fn ctx => fn meta => Scan.succeed (fn _ =>
+  meta |> NuBasics.apply_proc_naive @{thm dpr_auto_schema'} |> NuSys.accept_proc ctx)\<close> *)
+
+subsubsection \<open>let & local_value\<close>
+
+lemma op_let: " (\<And>p. p \<nuLinkL> A \<nuLinkR> a \<Longrightarrow> \<^bold>p\<^bold>r\<^bold>o\<^bold>c body p \<blangle> S\<heavy_comma> \<^bold>h\<^bold>e\<^bold>a\<^bold>p H \<longmapsto> X' \<brangle>) \<Longrightarrow>
+   \<^bold>p\<^bold>r\<^bold>o\<^bold>c op_let body \<blangle> S\<heavy_comma> a \<tycolon> A\<heavy_comma> \<^bold>h\<^bold>e\<^bold>a\<^bold>p H \<longmapsto> X' \<brangle>"
+  unfolding Procedure_def op_let_def by (auto simp add: nu_exps)
+
+lemma op_local_value: "v \<nuLinkL> A \<nuLinkR> a \<Longrightarrow> \<^bold>p\<^bold>r\<^bold>o\<^bold>c op_local_value v \<blangle> S\<heavy_comma> \<^bold>h\<^bold>e\<^bold>a\<^bold>p H \<longmapsto> S\<heavy_comma> a \<tycolon> A\<heavy_comma> \<^bold>h\<^bold>e\<^bold>a\<^bold>p H \<brangle>"
+  unfolding Procedure_def op_local_value_def by (auto simp add: nu_exps)
+
+ML_file "library/local_value.ML"
+
+\<nu>processor let_local_value 500 \<open>\<^bold>c\<^bold>u\<^bold>r\<^bold>r\<^bold>e\<^bold>n\<^bold>t blk [\<HH>] \<^bold>r\<^bold>e\<^bold>s\<^bold>u\<^bold>l\<^bold>t\<^bold>s \<^bold>i\<^bold>n (R\<heavy_comma> x \<tycolon> X\<heavy_comma> \<^bold>h\<^bold>e\<^bold>a\<^bold>p H)\<close> \<open>let open Parse in
+  fn ctx => fn sequent => (($$$ "\<rightarrow>" || $$$ "--") -- list1 binding) >> (fn (keyword,idts) => fn _ =>
+    Local_Value.mk_let (keyword = "--") (rev idts) sequent ctx
+) end\<close>
+
+
+subsubsection \<open>function call\<close>
+  \<comment> \<open>A function is the program function in the ordinary meaning that called by pushing stack frame, rarely inline
+    (whereas a procedure is generally inline), which is a procedure of \<^term>\<open>Void\<close> as its stack remainder so that
+    it can only access its arguments and never the stack remainder.
+    A function always corresponds an LLVM function, whereas other ordinary procedures are totally inline at the calling place generally
+      except some cases of optimization.
+    Only a function but no other ordinary procedure locates at a decided address in memory during the runtime,
+    so that has function pointers to it, and therefore can be indirectly called by the pointer. \<close>
+
+
+
+(* definition strip_end_tail :: " ('a::lrep \<times> void \<longmapsto> ('b::lrep \<times> void)) \<Rightarrow> 'a \<times> ('r::stack) \<longmapsto> ('b \<times> 'r)"
+  where "strip_end_tail f s = (case s of (a,r) \<Rightarrow> bind (f (a,void)) (\<lambda>(b,_). StatOn (b,r)))"
+lemma strip_end_tail: "\<^bold>p\<^bold>r\<^bold>o\<^bold>c f \<blangle> \<^bold>E\<^bold>N\<^bold>D\<heavy_comma> A \<longmapsto> \<^bold>E\<^bold>N\<^bold>D\<heavy_comma> B \<brangle> \<Longrightarrow> \<^bold>p\<^bold>r\<^bold>o\<^bold>c strip_end_tail f \<blangle> R\<heavy_comma> A \<longmapsto> R\<heavy_comma> B \<brangle>"
+  unfolding strip_end_tail_def Procedure_def bind_def by (auto 4 4)
+*)
+
+
+subsection \<open>Branches & Loops\<close>
+
+subsubsection \<open>sel\<close>
+
+lemma sel_\<nu>app:
+  "\<^bold>p\<^bold>r\<^bold>o\<^bold>c op_sel TYPE('a::lrep) \<blangle> R\<heavy_comma> a \<tycolon> T\<heavy_comma> b \<tycolon> T\<heavy_comma> c \<tycolon> \<bool>\<heavy_comma> \<^bold>h\<^bold>e\<^bold>a\<^bold>p Nothing \<longmapsto> R\<heavy_comma> (if c then a else b) \<tycolon> T\<heavy_comma> \<^bold>h\<^bold>e\<^bold>a\<^bold>p Nothing \<brangle> "
+  unfolding Procedure_def op_sel_def by (auto simp add: nu_exps)
+
+subsubsection \<open>if\<close>
+
+declare op_if_def[\<nu>instr]
+
+lemma if_\<nu>app:
+  "(cond \<longrightarrow> \<^bold>p\<^bold>r\<^bold>o\<^bold>c branch_true \<blangle> X \<longmapsto> Y\<^sub>T \<brangle>)
+    \<longrightarrow> SameNuTy Y\<^sub>T Y\<^sub>F
+    \<longrightarrow> (\<not> cond \<longrightarrow> \<^bold>p\<^bold>r\<^bold>o\<^bold>c branch_false \<blangle> X \<longmapsto> Y\<^sub>F \<brangle>)
+    \<longrightarrow> \<^bold>p\<^bold>r\<^bold>o\<^bold>c op_if TYPE('y::stack) branch_true branch_false \<blangle> X \<heavy_comma>^ cond \<tycolon> \<bool> \<longmapsto> (if cond then Y\<^sub>T else Y\<^sub>F) \<brangle>"
+  unfolding \<nu>def op_if_def by (auto simp add: nu_exps)
+(* text \<open>Despite the feasibility of divergence of \<nu>-types in the branch, i.e.
+  \<^term>\<open>\<^bold>p\<^bold>r\<^bold>o\<^bold>c op_if branch_true branch_false \<blangle> x \<tycolon> X \<heavy_comma>^ cond \<tycolon> \<bool> \<longmapsto> (if cond then y\<^sub>T else y\<^sub>F) \<tycolon> (if cond then Y\<^sub>T else Y\<^sub>F ) \<brangle>\<close>,
+  from the design of the programming principles, considering the role of \<nu>-types which encodes the invariant properties,
+  we prohibit the divergence of \<nu>-types.\<close> *)
+
+lemma [simp]: "(if P then \<tort_lbrace>x \<tycolon> X\<tort_rbrace> else \<tort_lbrace>y \<tycolon> Y\<tort_rbrace>) = \<tort_lbrace>(if P then x else y) \<tycolon> (if P then X else Y)\<tort_rbrace>" by simp
+lemma [simp]: "(if P then (a,b) else (a',b')) = ((if P then a else a'), (if P then b else b'))" by simp
+(* lemma AA: "(if P then A else B) = (\<lambda>x. if P then A x else B x)" by simp *)
+lemma [simp]: "(if P then (S\<heavy_comma> \<^bold>h\<^bold>e\<^bold>a\<^bold>p H) else (S'\<heavy_comma> \<^bold>h\<^bold>e\<^bold>a\<^bold>p H')) = ((if P then S else S')\<heavy_comma> \<^bold>h\<^bold>e\<^bold>a\<^bold>p (if P then H else H'))" by simp
+lemma [simp]: "(if P then (A\<heavy_comma> B) else (A'\<heavy_comma> B')) = ((if P then A else A')\<heavy_comma> (if P then B else B'))" by simp
+lemma [simp]: "(if P then (A \<heavy_asterisk> B) else (A' \<heavy_asterisk> B')) = ((if P then A else A') \<heavy_asterisk> (if P then B else B'))" by simp
+(* lemma [simp]: "(if P then (A \<^bold>a\<^bold>n\<^bold>d B) else (A' \<^bold>a\<^bold>n\<^bold>d B')) = ((if P then A else A') \<^bold>a\<^bold>n\<^bold>d (if P then B else B'))"  by auto *)
+lemma [simp]: "(if P then Labelled name T else Labelled name' T') = Labelled name (if P then T else T')" unfolding Labelled_def by simp
+lemma [simp]: "(if P then a \<R_arr_tail> x else a \<R_arr_tail> x') = a \<R_arr_tail> (if P then x else x')" by auto
+
+
+subsubsection \<open>do while\<close>
+
+lemma SemDoWhile_deterministic:
+  assumes "SemDoWhile c s s1"
+      and "SemDoWhile c s s2"
+    shows "s1 = s2"
+proof -
+  have "SemDoWhile c s s1 \<Longrightarrow> (\<forall>s2. SemDoWhile c s s2 \<longrightarrow> s1 = s2)"
+    by (induct rule: SemDoWhile.induct) (subst SemDoWhile.simps, simp)+
+  thus ?thesis
+    using assms by simp
+qed
+
+lemma SemDoWhile_deterministic2: " SemDoWhile body s x \<Longrightarrow> The ( SemDoWhile body s) = x"
+  using SemDoWhile_deterministic by blast
+
+declare Heap'_expn[simp del]
+lemma "__DoWhile___\<nu>app":
+  "(\<forall>x. \<^bold>p\<^bold>r\<^bold>e\<^bold>m\<^bold>i\<^bold>s\<^bold>e P x \<longrightarrow> \<^bold>p\<^bold>r\<^bold>o\<^bold>c body \<blangle> X x \<longmapsto> \<exists>* x'. X x' \<heavy_comma>^ P x' \<tycolon> \<bool> \<brangle>)
+    \<longrightarrow> \<^bold>p\<^bold>r\<^bold>e\<^bold>m\<^bold>i\<^bold>s\<^bold>e P x \<longrightarrow> \<^bold>p\<^bold>r\<^bold>o\<^bold>c op_do_while TYPE('a::stack) body \<blangle> X x \<longmapsto> \<exists>* x'. X x' \<and>\<^sup>s (\<not> P x') \<brangle>"
+(*  for X :: "(heap \<times> 'a::lrep, 'b) \<nu>" *)
+  unfolding op_do_while_def Procedure_def Auto_def
+  apply (auto simp add: SemDoWhile_deterministic2 nu_exps Heap'_Stack_Front Heap'_ExSet Heap'_Addition)
+  subgoal for a b xa H
+    apply (rotate_tac 2)
+    by (induct  body "(a, b)" xa arbitrary: a b x rule: SemDoWhile.induct) (auto 0 7 simp add: nu_exps)
+  done
+declare Heap'_expn[simp]
+
+
+lemma do_while_\<nu>app:
+  "Variant_Cast vars S H S' H' \<longrightarrow>
+  \<^bold>p\<^bold>a\<^bold>r\<^bold>a\<^bold>m cond \<longrightarrow>
+  \<^bold>p\<^bold>r\<^bold>e\<^bold>m\<^bold>i\<^bold>s\<^bold>e cond vars \<longrightarrow>
+  (\<forall>x. \<^bold>p\<^bold>r\<^bold>e\<^bold>m\<^bold>i\<^bold>s\<^bold>e cond x \<longrightarrow> \<^bold>p\<^bold>r\<^bold>o\<^bold>c body \<blangle> S' x\<heavy_comma> \<^bold>h\<^bold>e\<^bold>a\<^bold>p H' x \<longmapsto> \<exists>* x'. (S' x' \<heavy_comma> cond x' \<tycolon> \<bool>\<heavy_comma> \<^bold>h\<^bold>e\<^bold>a\<^bold>p H' x') \<brangle>) \<longrightarrow>
+  \<^bold>p\<^bold>r\<^bold>o\<^bold>c op_do_while TYPE('a::stack)  body \<blangle> S\<heavy_comma> \<^bold>h\<^bold>e\<^bold>a\<^bold>p H \<longmapsto> \<exists>* x'. (S' x'\<heavy_comma> \<^bold>h\<^bold>e\<^bold>a\<^bold>p H' x') \<and>\<^sup>s (\<not> cond x') \<brangle>"
+  unfolding Variant_Cast_def Premise_def apply simp
+  using "__DoWhile___\<nu>app"[of "cond" _ "(\<lambda>x. S' x\<heavy_comma> \<^bold>h\<^bold>e\<^bold>a\<^bold>p H' x)", unfolded Premise_def, simplified] by blast
+
+
+subsubsection \<open>while\<close>
+
+proc while: \<open>S'\<heavy_comma> \<^bold>h\<^bold>e\<^bold>a\<^bold>p H'\<close> \<longmapsto> \<open>\<exists>* x. (S x\<heavy_comma> \<^bold>h\<^bold>e\<^bold>a\<^bold>p H x) \<and>\<^sup>s (\<not> cond x)\<close>
+  for S' :: " 'b::stack set"
+  requires [unfolded Variant_Cast_def, simp]: "Variant_Cast vars S' H' S H"
+    and Cond_\<nu>app: "\<forall>x. \<^bold>p\<^bold>r\<^bold>o\<^bold>c Cond \<blangle> S x\<heavy_comma> \<^bold>h\<^bold>e\<^bold>a\<^bold>p H x \<longmapsto> \<exists>* x'. (S x'\<heavy_comma> cond x' \<tycolon> \<bool>\<heavy_comma> \<^bold>h\<^bold>e\<^bold>a\<^bold>p H x')\<brangle>"
+    and Body_\<nu>app: "\<forall>x. \<^bold>p\<^bold>r\<^bold>e\<^bold>m\<^bold>i\<^bold>s\<^bold>e cond x \<longrightarrow> \<^bold>p\<^bold>r\<^bold>o\<^bold>c Body \<blangle> S x\<heavy_comma> \<^bold>h\<^bold>e\<^bold>a\<^bold>p H x \<longmapsto> \<exists>* x'. (S x'\<heavy_comma> \<^bold>h\<^bold>e\<^bold>a\<^bold>p H x') \<brangle>"
+  \<bullet> Cond if \<medium_left_bracket> do_while x' \<open>cond x'\<close> \<medium_left_bracket> Body Cond \<medium_right_bracket> subj \<open>\<not> cond x'\<close> \<medium_right_bracket> \<medium_left_bracket> \<medium_right_bracket>
+  finish
+
+
+subsubsection \<open>recursion\<close>
+
+lemma SemRec_IR: "SemRec F x y \<Longrightarrow> SemRec (F o F) x y"
+  by (induct rule: SemRec.induct, rule SemRec_I0, simp)
+
+lemma SemRec_deterministic:
+  assumes "SemRec c s s1" and "SemRec c s s2" shows "s1 = s2"
+proof -
+  have "SemRec c s s1 \<Longrightarrow> (\<forall>s2. SemRec c s s2 \<longrightarrow> s1 = s2)"
+    apply (induct rule: SemRec.induct)
+     apply clarify
+    subgoal for F a b y s2 apply (rotate_tac 1)
+      apply (induct rule: SemRec.induct) by auto 
+    apply clarify apply (blast intro: SemRec_IR) done
+  thus ?thesis using assms by simp
+qed
+
+lemma SemRec_deterministic2: " SemRec body s x \<Longrightarrow> The ( SemRec body s) = x"
+  using SemRec_deterministic by blast
+
+
+declare Heap'_expn[simp del]
+lemma op_recursion':
+  "(\<And>g x'. (\<forall>x''. \<^bold>p\<^bold>r\<^bold>o\<^bold>c g \<blangle> X x'' \<longmapsto> Y x'' \<brangle>) \<longrightarrow> \<^bold>p\<^bold>r\<^bold>o\<^bold>c F g \<blangle> X x' \<longmapsto> Y x' \<brangle>) \<Longrightarrow>
+    (\<forall>x. \<^bold>p\<^bold>r\<^bold>o\<^bold>c op_recursion' F \<blangle> X x \<longmapsto> Y x \<brangle>)"
+  (* for X :: "'b \<Rightarrow> (heap \<times> 'a::lrep, 'b) \<nu>" *)
+  unfolding op_recursion'_def Procedure_def Function_def atomize_all
+  apply (auto simp add: SemRec_deterministic2)
+  subgoal for x a b xa apply (rotate_tac 1) apply (induct rule:  SemRec.induct) by (auto 0 6) done
+declare Heap'_expn[simp]
+
+lemma op_recursion:
+  "(\<And>g x'. (\<forall>x''. \<^bold>f\<^bold>u\<^bold>n\<^bold>c g \<blangle> X x'' \<longmapsto> Y x'' \<brangle>) \<longrightarrow> \<^bold>p\<^bold>r\<^bold>o\<^bold>c F g \<blangle> X x' \<longmapsto> Y x' \<brangle>) \<Longrightarrow>
+    (\<forall>x. \<^bold>f\<^bold>u\<^bold>n\<^bold>c op_recursion UNIQ_ID TYPE('x::lrep) TYPE('y::lrep) F \<blangle> X x \<longmapsto> Y x \<brangle>)"
+  unfolding op_recursion_def func_ALL Function_def apply simp
+  using op_recursion'[of X Y "F o func", simplified] .
+
+hide_const op_recursion'
+hide_fact op_recursion'
+
+
+section \<open>Arithmetic instructions\<close>
+
+\<nu>overloads "+" and round_add and "<" and "\<le>" and "-" and "/" and "=" and "not"
+
+subsection \<open>Integer arithmetic\<close>
+
+subsubsection \<open>constant\<close>
+
+(* theorem const_nat_\<nu>app: "\<^bold>p\<^bold>r\<^bold>o\<^bold>c op_const_int TYPE('w::len) c \<blangle> R\<heavy_comma> \<^bold>h\<^bold>e\<^bold>a\<^bold>p Nothing \<longmapsto> R \<heavy_comma> c \<tycolon> \<nat>['w]\<heavy_comma> \<^bold>h\<^bold>e\<^bold>a\<^bold>p Nothing \<brangle>"
+  unfolding \<nu>def op_const_int_def apply (auto simp add: nu_exps) *)
+(* theorem const_nat_round_\<nu>app: "\<^bold>p\<^bold>r\<^bold>o\<^bold>c op_const_int TYPE('w::len) (of_nat n) \<blangle> R \<longmapsto> R \<heavy_comma> n \<tycolon> \<nat>\<^sup>r['w] \<brangle>"
+  unfolding \<nu>def op_const_int_def by auto *)
+
+lemma [\<nu>intro]:
+  "\<^bold>p\<^bold>r\<^bold>e\<^bold>m\<^bold>i\<^bold>s\<^bold>e (numeral x :: nat) < 2^LENGTH('w) \<Longrightarrow>
+   \<^bold>c\<^bold>o\<^bold>n\<^bold>s\<^bold>t\<^bold>r\<^bold>u\<^bold>c\<^bold>t ((numeral x) \<tycolon> \<nat>['w]) \<^bold>b\<^bold>y \<^bold>p\<^bold>r\<^bold>o\<^bold>c op_const_int TYPE('w::len) (numeral x)
+    \<blangle> R\<heavy_comma> \<^bold>h\<^bold>e\<^bold>a\<^bold>p H \<longmapsto> R \<heavy_comma> (numeral x) \<tycolon> \<nat>['w]\<heavy_comma> \<^bold>h\<^bold>e\<^bold>a\<^bold>p H \<brangle>"
+  unfolding op_const_int_def \<nu>def including show_more1 by (auto simp add: nu_exps) (metis mod_if unat_bintrunc unat_numeral)
+  \<comment> \<open>Only literal number could be constructed automatically\<close>
+
+lemma [\<nu>intro]:
+  "\<^bold>c\<^bold>o\<^bold>n\<^bold>s\<^bold>t\<^bold>r\<^bold>u\<^bold>c\<^bold>t (0 \<tycolon> \<nat>['w]) \<^bold>b\<^bold>y \<^bold>p\<^bold>r\<^bold>o\<^bold>c op_const_int TYPE('w::len) 0
+    \<blangle> R\<heavy_comma> \<^bold>h\<^bold>e\<^bold>a\<^bold>p H \<longmapsto> R \<heavy_comma> 0 \<tycolon> \<nat>['w]\<heavy_comma> \<^bold>h\<^bold>e\<^bold>a\<^bold>p H \<brangle>"
+  unfolding AutoConstruct_def \<nu>def op_const_int_def by (auto simp add: nu_exps)
+
+lemma [\<nu>intro]:
+  "\<^bold>c\<^bold>o\<^bold>n\<^bold>s\<^bold>t\<^bold>r\<^bold>u\<^bold>c\<^bold>t (1 \<tycolon> \<nat>['w]) \<^bold>b\<^bold>y \<^bold>p\<^bold>r\<^bold>o\<^bold>c op_const_int TYPE('w::len) 1
+    \<blangle> R\<heavy_comma> \<^bold>h\<^bold>e\<^bold>a\<^bold>p H \<longmapsto> R\<heavy_comma> 1 \<tycolon> \<nat>['w]\<heavy_comma> \<^bold>h\<^bold>e\<^bold>a\<^bold>p H \<brangle>"
+  unfolding AutoConstruct_def \<nu>def op_const_int_def by (auto simp add: nu_exps)
+
+lemma [\<nu>intro]:
+  "\<^bold>p\<^bold>r\<^bold>e\<^bold>m\<^bold>i\<^bold>s\<^bold>e (numeral x :: nat) < 2^LENGTH('w) \<Longrightarrow>
+   \<^bold>c\<^bold>o\<^bold>n\<^bold>s\<^bold>t\<^bold>r\<^bold>u\<^bold>c\<^bold>t ((numeral x) \<tycolon> \<nat>\<^sup>r['w]) \<^bold>b\<^bold>y \<^bold>p\<^bold>r\<^bold>o\<^bold>c op_const_int TYPE('w::len) (numeral x)
+    \<blangle> R\<heavy_comma> \<^bold>h\<^bold>e\<^bold>a\<^bold>p H \<longmapsto> R\<heavy_comma> (numeral x) \<tycolon> \<nat>\<^sup>r['w]\<heavy_comma> \<^bold>h\<^bold>e\<^bold>a\<^bold>p H \<brangle>"
+  unfolding op_const_int_def \<nu>def including show_more1 by (auto simp add: nu_exps)
+
+lemma [\<nu>intro]:
+  "\<^bold>c\<^bold>o\<^bold>n\<^bold>s\<^bold>t\<^bold>r\<^bold>u\<^bold>c\<^bold>t (0 \<tycolon> \<nat>\<^sup>r['w]) \<^bold>b\<^bold>y \<^bold>p\<^bold>r\<^bold>o\<^bold>c op_const_int TYPE('w::len) 0 \<blangle> R\<heavy_comma> \<^bold>h\<^bold>e\<^bold>a\<^bold>p H \<longmapsto> R\<heavy_comma> 0 \<tycolon> \<nat>\<^sup>r['w]\<heavy_comma> \<^bold>h\<^bold>e\<^bold>a\<^bold>p H \<brangle>"
+  unfolding op_const_int_def \<nu>def including show_more1 by (auto simp add: nu_exps)
+
+lemma [\<nu>intro]:
+  "\<^bold>c\<^bold>o\<^bold>n\<^bold>s\<^bold>t\<^bold>r\<^bold>u\<^bold>c\<^bold>t (1 \<tycolon> \<nat>\<^sup>r['w]) \<^bold>b\<^bold>y \<^bold>p\<^bold>r\<^bold>o\<^bold>c op_const_int TYPE('w::len) 1 \<blangle> R\<heavy_comma> \<^bold>h\<^bold>e\<^bold>a\<^bold>p H \<longmapsto> R\<heavy_comma> 1 \<tycolon> \<nat>\<^sup>r['w]\<heavy_comma> \<^bold>h\<^bold>e\<^bold>a\<^bold>p H \<brangle>"
+  unfolding op_const_int_def \<nu>def including show_more1 by (auto simp add: nu_exps)
+
+
+lemma [\<nu>intro 1100]:
+  "\<^bold>c\<^bold>o\<^bold>n\<^bold>s\<^bold>t\<^bold>r\<^bold>u\<^bold>c\<^bold>t ((numeral x) \<tycolon> \<nat>[size_t]) \<^bold>b\<^bold>y \<^bold>p\<^bold>r\<^bold>o\<^bold>c op_const_size_t (numeral x)
+    \<blangle> R\<heavy_comma> \<^bold>h\<^bold>e\<^bold>a\<^bold>p H \<longmapsto> R\<heavy_comma> (numeral x) \<tycolon> \<nat>[size_t]\<heavy_comma> \<^bold>h\<^bold>e\<^bold>a\<^bold>p H \<brangle>"
+  unfolding op_const_size_t_def \<nu>def by (auto simp add: nu_exps nat_take_bit_eq take_bit_nat_eq_self_iff)
+
+
+(* schematic_goal "\<^bold>c\<^bold>o\<^bold>n\<^bold>s\<^bold>t\<^bold>r\<^bold>u\<^bold>c\<^bold>t 3 \<^bold>b\<^bold>y \<^bold>p\<^bold>r\<^bold>o\<^bold>c ?f
+  \<blangle>\<flower_L>\<medium_left_bracket> A \<flower_L>\<flower>\<flower_R>X\<medium_right_bracket>\<flower_R>   \<longmapsto> ?T \<brangle>" by (rule \<nu>intro) *)
+
+subsubsection \<open>plus\<close>
+
+(* instantiation typing :: (lrep, plus) plus begin
+definition plus_typing :: "('a,'b) typing \<Rightarrow> ('a,'b) typing \<Rightarrow> ('a,'b) typing"
+  where "nu_of a = nu_of b \<Longrightarrow> plus_typing a b = (case a of xa \<tycolon> Na \<Rightarrow> case b of xb \<tycolon> Nb \<Rightarrow> xa + xb \<tycolon> Na)"
+lemma [simp]: "(x \<tycolon> N) + (y \<tycolon> N) = (x + y \<tycolon> N)" using plus_typing_def by auto
+instance by standard
+end *)
+
+theorem add_nat_\<nu>app[\<nu>overload +]:
+  "\<^bold>p\<^bold>r\<^bold>e\<^bold>m\<^bold>i\<^bold>s\<^bold>e x + y < 2^LENGTH('b::len) \<longrightarrow>
+    \<^bold>p\<^bold>r\<^bold>o\<^bold>c op_add TYPE('b) \<blangle> R\<heavy_comma> x \<tycolon> \<nat>['b] \<heavy_comma> y \<tycolon> \<nat>['b]\<heavy_comma> \<^bold>h\<^bold>e\<^bold>a\<^bold>p Nothing \<longmapsto> R\<heavy_comma> x + y \<tycolon> \<nat>['b]\<heavy_comma> \<^bold>h\<^bold>e\<^bold>a\<^bold>p Nothing \<brangle>"
+  unfolding op_add_def Procedure_def by (auto simp add: of_nat_inverse nu_exps)
+
+theorem add_nat_round[\<nu>overload +]:
+  "\<^bold>p\<^bold>r\<^bold>o\<^bold>c op_add TYPE('b) \<blangle> R\<heavy_comma> x \<tycolon> \<nat>\<^sup>r['b::len]\<heavy_comma> y \<tycolon> \<nat>\<^sup>r['b]\<heavy_comma> \<^bold>h\<^bold>e\<^bold>a\<^bold>p Nothing \<longmapsto> R\<heavy_comma> (x + y) \<tycolon> \<nat>\<^sup>r['b]\<heavy_comma> \<^bold>h\<^bold>e\<^bold>a\<^bold>p Nothing \<brangle>"
+  unfolding op_add_def Procedure_def by (auto simp add: nu_exps)
+
+(* theorem add_nat_mod[\<nu>overload round_add]:
+    "\<^bold>p\<^bold>r\<^bold>o\<^bold>c op_add (LENGTH('b)) \<blangle>\<^bold>E\<^bold>N\<^bold>D \<RR> \<heavy_comma> y \<tycolon> \<nat>['b::len] \<heavy_comma> x \<tycolon> \<nat>['b] \<longmapsto> \<^bold>E\<^bold>N\<^bold>D \<RR> \<heavy_comma> ((x + y) mod 2^(LENGTH('b))) \<tycolon> \<nat>['b]  \<brangle>"
+  unfolding op_add_def Procedure_def by (auto simp add: unat_word_ariths)
+*)
+
+subsubsection \<open>subtraction\<close>
+
+theorem sub_nat_\<nu>app[\<nu>overload -]:
+    "\<^bold>p\<^bold>r\<^bold>e\<^bold>m\<^bold>i\<^bold>s\<^bold>e y \<le> x \<longrightarrow>
+    \<^bold>p\<^bold>r\<^bold>o\<^bold>c op_sub TYPE('w::len) \<blangle> R\<heavy_comma> x \<tycolon> \<nat>['w] \<heavy_comma> y \<tycolon> \<nat>['w]\<heavy_comma> \<^bold>h\<^bold>e\<^bold>a\<^bold>p Nothing \<longmapsto> R\<heavy_comma> x - y \<tycolon> \<nat>['w]\<heavy_comma> \<^bold>h\<^bold>e\<^bold>a\<^bold>p Nothing \<brangle>"
+  unfolding \<nu>def op_sub_def by (auto simp add: nu_exps) (meson unat_sub_if_size)
+
+
+subsubsection \<open>division\<close>
+
+theorem udiv_nat_\<nu>app[\<nu>overload /]:
+    "\<^bold>p\<^bold>r\<^bold>o\<^bold>c op_udiv TYPE('w::len) \<blangle> R\<heavy_comma> x \<tycolon> \<nat>['w] \<heavy_comma> y \<tycolon> \<nat>['w]\<heavy_comma> \<^bold>h\<^bold>e\<^bold>a\<^bold>p Nothing \<longmapsto> R\<heavy_comma> x div y \<tycolon> \<nat>['w]\<heavy_comma> \<^bold>h\<^bold>e\<^bold>a\<^bold>p Nothing \<brangle>"
+  unfolding \<nu>def op_udiv_def by (auto simp add: nu_exps) (meson unat_div)
+
+subsubsection \<open>less\<close>
+
+theorem op_lt_\<nu>app[\<nu>overload <]:
+    "\<^bold>p\<^bold>r\<^bold>o\<^bold>c op_lt TYPE('w::len) \<blangle> R\<heavy_comma> x \<tycolon> \<nat>['w]\<heavy_comma> y \<tycolon> \<nat>['w]\<heavy_comma> \<^bold>h\<^bold>e\<^bold>a\<^bold>p Nothing \<longmapsto> R\<heavy_comma> (x < y) \<tycolon> \<bool>\<heavy_comma> \<^bold>h\<^bold>e\<^bold>a\<^bold>p Nothing \<brangle>"
+  unfolding \<nu>def op_lt_def by (auto simp add: word_less_nat_alt nu_exps)
+
+theorem op_le_\<nu>app[\<nu>overload \<le>]:
+    "\<^bold>p\<^bold>r\<^bold>o\<^bold>c op_le TYPE('w::len) \<blangle> R\<heavy_comma> x \<tycolon> \<nat>['w]\<heavy_comma> y \<tycolon> \<nat>['w]\<heavy_comma> \<^bold>h\<^bold>e\<^bold>a\<^bold>p Nothing \<longmapsto> R\<heavy_comma> (x \<le> y) \<tycolon> \<bool>\<heavy_comma> \<^bold>h\<^bold>e\<^bold>a\<^bold>p Nothing \<brangle>"
+  unfolding \<nu>def op_le_def by (auto simp add: word_le_nat_alt nu_exps)
+
+subsubsection \<open>bit-wise not\<close>
+
+lemma boolean_not_\<nu>app[\<nu>overload not]:
+    "\<^bold>p\<^bold>r\<^bold>o\<^bold>c op_not TYPE(1) \<blangle> R\<heavy_comma> x \<tycolon> \<bool>\<heavy_comma> \<^bold>h\<^bold>e\<^bold>a\<^bold>p Nothing \<longmapsto> R\<heavy_comma> \<not> x \<tycolon> \<bool>\<heavy_comma> \<^bold>h\<^bold>e\<^bold>a\<^bold>p Nothing \<brangle>"
+  unfolding Procedure_def op_not_def apply (auto simp add: lrep_exps nu_exps)
+  by (metis even_take_bit_eq even_zero iszero_def odd_numeral one_neq_zero)
+
+subsubsection \<open>equal\<close>
+
+theorem op_equal[\<nu>overload =]:
+  "\<nu>Equal N P eq \<longrightarrow> \<^bold>p\<^bold>r\<^bold>e\<^bold>m\<^bold>i\<^bold>s\<^bold>e P a b \<longrightarrow> \<^bold>p\<^bold>r\<^bold>o\<^bold>c op_equal \<blangle> R\<heavy_comma> a \<tycolon> N\<heavy_comma> b \<tycolon> N\<heavy_comma> \<^bold>h\<^bold>e\<^bold>a\<^bold>p Nothing \<longmapsto> R\<heavy_comma> eq a b \<tycolon> \<bool>\<heavy_comma> \<^bold>h\<^bold>e\<^bold>a\<^bold>p Nothing \<brangle>"
+  unfolding \<nu>def op_equal_def by (auto 0 6 simp add: nu_exps)
+
+section \<open>Tuple Operations\<close>
+
+subsection \<open>Tuple construction & destruction\<close>
+
+subsubsection \<open>cons_tup\<close>
+
+theorem tup_\<nu>app:
+    "\<^bold>p\<^bold>r\<^bold>o\<^bold>c cons_tup TYPE('a::field_list) \<blangle> R \<heavy_comma> x \<tycolon> X\<heavy_comma> \<^bold>h\<^bold>e\<^bold>a\<^bold>p Nothing \<longmapsto> R \<heavy_comma> x \<tycolon> \<lbrace> X \<rbrace> \<heavy_comma> \<^bold>h\<^bold>e\<^bold>a\<^bold>p Nothing \<brangle>"
+  unfolding cons_tup_def Procedure_def by (simp add: pair_forall nu_exps)
+
+subsubsection \<open>op_dest_tup\<close>
+
+theorem det_\<nu>app:
+    "\<^bold>p\<^bold>r\<^bold>o\<^bold>c op_dest_tup \<blangle> R\<heavy_comma> x \<tycolon> \<lbrace> X \<rbrace>\<heavy_comma> \<^bold>h\<^bold>e\<^bold>a\<^bold>p Nothing \<longmapsto> R\<heavy_comma> x \<tycolon> X\<heavy_comma> \<^bold>h\<^bold>e\<^bold>a\<^bold>p Nothing \<brangle>"
+  unfolding Procedure_def op_dest_tup_def by (simp add: tuple_forall pair_forall nu_exps)
+
+subsection \<open>Field Index\<close>
+
+definition FieldIndex :: " ('a,'a,'ax,'ax) index \<Rightarrow> ('ax::lrep,'bx) \<nu> \<Rightarrow> ('a::lrep,'b) \<nu> \<Rightarrow> ('b \<Rightarrow> 'bx) \<Rightarrow> (('bx \<Rightarrow> 'bx) \<Rightarrow> 'b \<Rightarrow> 'b) \<Rightarrow>bool"
+  where "FieldIndex adr X A gt mp \<longleftrightarrow> (\<forall>a f. \<^bold>i\<^bold>n\<^bold>d\<^bold>e\<^bold>x adr \<blangle> \<tort_lbrace>gt a \<tycolon> X\<tort_rbrace> \<^bold>@ \<tort_lbrace>a \<tycolon> A\<tort_rbrace> \<longmapsto> \<tort_lbrace>f (gt a) \<tycolon> X\<tort_rbrace> \<^bold>@ \<tort_lbrace>mp f a \<tycolon> A\<tort_rbrace> \<brangle>)"
+
+lemma FieldIndex_here: "FieldIndex index_here X X id id"
+  unfolding FieldIndex_def \<nu>index_def index_here_def by auto
+lemma FieldIndex_left: "FieldIndex f X A gt mp \<Longrightarrow> FieldIndex (index_left f) X (A \<cross_product> R) (gt o fst) (apfst o mp)"
+  unfolding FieldIndex_def \<nu>index_def index_left_def by (auto simp add: nu_exps)
+lemma FieldIndex_right: "FieldIndex f X A gt mp \<Longrightarrow> FieldIndex (index_right f) X (R \<cross_product> A) (gt o snd) (apsnd o mp)"
+  unfolding FieldIndex_def \<nu>index_def index_right_def by (auto simp add: nu_exps)
+
+lemma FieldIndex_tupl: "FieldIndex f X A gt mp \<Longrightarrow> FieldIndex (index_enter_tup f) X \<lbrace> A \<rbrace> gt mp"
+  unfolding FieldIndex_def \<nu>index_def index_enter_tup_def by (auto simp add: tuple_forall nu_exps)
+
+\<nu>processor field_index 110 \<open>FieldIndex f X \<lbrace> A \<rbrace> gt mp \<Longrightarrow> PROP P\<close> \<open>fn ctx => fn major => Parse.nat >> (fn i => fn _ =>
+  let open NuBasics NuHelp
+    val arity = Logic.dest_implies (prop_of major) |> #1
+        |> dest_Trueprop |> dest_quinop \<^const_name>\<open>FieldIndex\<close> |> #3
+        |> dest_monop \<^const_name>\<open>NuTuple\<close> |> strip_binop_r \<^const_name>\<open>Fusion\<close> |> length
+    val path1 = funpow (i-1) (fn th => th RS @{thm FieldIndex_right})
+        (@{thm FieldIndex_here}
+              |> (fn th => if arity = i then th else th RS @{thm FieldIndex_left}))
+  in 
+    (path1 RS (@{thm FieldIndex_tupl} RS major), ctx)
+  end)\<close>
+
+subsection \<open>Field Accessing\<close>
+
+lemma
+  "\<^bold>i\<^bold>n\<^bold>d\<^bold>e\<^bold>x idx \<blangle> X \<^bold>@ A \<brangle> \<Longrightarrow>
+    \<^bold>p\<^bold>r\<^bold>o\<^bold>c op_get_tuple idx TYPE('a::field_list) \<blangle> R\<heavy_comma> A\<heavy_comma> \<^bold>h\<^bold>e\<^bold>a\<^bold>p Nothing \<longmapsto> R\<heavy_comma> X\<heavy_comma> \<^bold>h\<^bold>e\<^bold>a\<^bold>p Nothing \<brangle> "
+  unfolding \<nu>index_def \<nu>def pair_forall op_get_tuple_def tuple_forall by simp
+
+lemma "\<^bold>i\<^bold>n\<^bold>d\<^bold>e\<^bold>x idx \<blangle> X \<^bold>@ A \<longmapsto> Y \<^bold>@ B \<brangle> \<Longrightarrow>
+  \<^bold>p\<^bold>r\<^bold>o\<^bold>c op_set_tuple idx TYPE('a::field_list) TYPE('y::lrep) \<blangle> R\<heavy_comma> A\<heavy_comma> Y\<heavy_comma> \<^bold>h\<^bold>e\<^bold>a\<^bold>p Nothing \<longmapsto> R\<heavy_comma> B\<heavy_comma> \<^bold>h\<^bold>e\<^bold>a\<^bold>p Nothing \<brangle> "
+  unfolding \<nu>index_def \<nu>def pair_forall op_set_tuple_def by simp
+
+
+section \<open>Memory & Pointer Operations\<close>
+
+subsection \<open>Pointer Arithmetic\<close>
+
+(* theorem op_shift_pointer_raw[\<nu>overload +]:
+  "\<^bold>p\<^bold>r\<^bold>o\<^bold>c op_shift_pointer ty \<blangle> R\<heavy_comma> addr \<tycolon> RawPointer\<heavy_comma> delta \<tycolon> Identity\<heavy_comma> \<^bold>h\<^bold>e\<^bold>a\<^bold>p H \<longmapsto>
+      R\<heavy_comma> shift_addr addr (delta * of_nat (size_of ty)) \<tycolon> RawPointer\<heavy_comma> \<^bold>h\<^bold>e\<^bold>a\<^bold>p H \<brangle>"
+  unfolding \<nu>def op_shift_pointer_def by (cases addr) (simp add: lrep_exps) *)
+  
+theorem op_shift_pointer[\<nu>overload +]:
+  "\<^bold>p\<^bold>r\<^bold>e\<^bold>m\<^bold>i\<^bold>s\<^bold>e address_llty addr = LLTY('a::lrep) \<Longrightarrow> \<^bold>p\<^bold>r\<^bold>e\<^bold>m\<^bold>i\<^bold>s\<^bold>e offset_of addr + delta \<le> address_len addr \<Longrightarrow>
+  \<^bold>p\<^bold>r\<^bold>o\<^bold>c op_shift_pointer TYPE('a::lrep) \<blangle> R\<heavy_comma> addr \<tycolon> Pointer\<heavy_comma> delta \<tycolon> \<nat>[size_t]\<heavy_comma> \<^bold>h\<^bold>e\<^bold>a\<^bold>p Nothing \<longmapsto>
+      R\<heavy_comma> addr ||+ delta \<tycolon> Pointer\<heavy_comma> \<^bold>h\<^bold>e\<^bold>a\<^bold>p Nothing \<brangle>"
+  unfolding \<nu>def op_shift_pointer_def by (cases addr) (auto simp add: lrep_exps same_addr_offset_def nu_exps)
+
+
+theorem op_shift_pointer_slice[ unfolded Separation_assoc, \<nu>overload split ]:
+  "\<^bold>p\<^bold>r\<^bold>e\<^bold>m\<^bold>i\<^bold>s\<^bold>e n < length xs \<longrightarrow>
+  \<^bold>p\<^bold>r\<^bold>o\<^bold>c op_shift_pointer TYPE('p) \<blangle> R\<heavy_comma> addr \<tycolon> Pointer\<heavy_comma> n \<tycolon> \<nat>[size_t]\<heavy_comma> \<^bold>h\<^bold>e\<^bold>a\<^bold>p addr \<R_arr_tail> xs \<tycolon> Array T
+      \<longmapsto> R\<heavy_comma> addr ||+ n \<tycolon> Pointer\<heavy_comma> \<^bold>h\<^bold>e\<^bold>a\<^bold>p (addr \<R_arr_tail> take n xs \<tycolon> Array T \<heavy_asterisk> shift_addr addr n \<R_arr_tail> drop n xs \<tycolon> Array T) \<brangle>"
+  for T :: "('p::field, 'x) \<nu>"
+  unfolding \<nu>def op_shift_pointer_def Array_def Heap_Divider_def apply (cases addr)
+  apply (auto simp add: lrep_exps same_addr_offset_def raw_offset_of_def distrib_right nu_exps
+        add.commute add.left_commute intro: heap_split_id)
+  subgoal for x1 x2 aa b H h1 h2
+    by (rule heap_split_id, simp, rule heap_split_by_addr_set[of _ _ "{(x1 |+ x2 + i) | i. i < n}"]) (auto simp add: nu_exps)
+  done
+
+(*
+theorem op_slice_merge[\<nu>overload merge]:
+  "\<^bold>p\<^bold>r\<^bold>e\<^bold>m\<^bold>i\<^bold>s\<^bold>e shift_addr addr1 (length xs1) = addr2 \<longrightarrow>
+  \<^bold>p\<^bold>r\<^bold>o\<^bold>c op_drop \<blangle> \<^bold>E\<^bold>N\<^bold>D R\<heavy_comma> addr1 \<R_arr_tail> xs1 \<tycolon> Slice T\<heavy_comma> addr2 \<R_arr_tail> xs2 \<tycolon> Slice T
+      \<longmapsto> \<^bold>E\<^bold>N\<^bold>D R\<heavy_comma> addr1 \<R_arr_tail> xs1 @ xs2 \<tycolon> Slice T \<brangle>"
+  unfolding \<nu>def op_drop_def apply (cases addr1; cases addr2)
+  apply (auto 0 0 simp add: lrep_exps nth_append)
+  by (metis add.assoc add_diff_inverse_nat diff_add_inverse diff_less_mono not_le
+*)
+subsection \<open>Allocation\<close>
+
+
+lemma malloc_split: "Heap h \<Longrightarrow> P h (heap_assignN n v (malloc h) Map.empty) \<Longrightarrow>
+    \<exists>h1 h2. heap_assignN n v (malloc h) h = h1 ++ h2 \<and> dom h1 \<perpendicular> dom h2 \<and> P h1 h2"
+  apply (rule exI[of _ h], rule exI[of _ "heap_assignN n v (malloc h) Map.empty"], simp)
+  subgoal premises prems
+    unfolding heap_assignN_def using prems(1)
+    by (simp add: map_add_def fun_eq_iff resource_key_forall disjoint_rewL memaddr_forall dom_def
+          malloc option.case_eq_if) done
+
+(* lemma heap_assignN_subset: "Heap h \<Longrightarrow> h \<subseteq>\<^sub>m heap_assignN n v (malloc h) h"
+  unfolding heap_assignN_def map_le_def Ball_def by (simp add: malloc2 resource_key_forall memaddr_forall) *)
+
+lemma [intro]: "Heap h \<Longrightarrow> Heap (heap_assignN n v seg h)" proof -
+  have "AvailableSegments h \<subseteq> {seg} \<union> AvailableSegments (heap_assignN n v seg h)"
+    unfolding AvailableSegments_def heap_assignN_def by auto 
+  then show "Heap h \<Longrightarrow> Heap (heap_assignN n v seg h)" 
+    unfolding Heap_def using infinite_super by auto
+qed
+
+lemma heap_assignN_eval: "v \<in> T \<Longrightarrow> i < n \<Longrightarrow> heap_assignN n (Some (deepize v)) seg h \<^bold>a\<^bold>t (seg |+ i) \<^bold>i\<^bold>s T"
+  unfolding MemAddrState_def addr_allocated_def heap_assignN_def by auto
+
+
+
+      
+theorem alloc_array_\<nu>app:
+  "\<^bold>p\<^bold>a\<^bold>r\<^bold>a\<^bold>m N \<Longrightarrow> \<nu>Zero N zero \<Longrightarrow> \<^bold>p\<^bold>r\<^bold>o\<^bold>c op_alloc TYPE('x)
+      \<blangle> R\<heavy_comma> n \<tycolon> \<nat>[size_t] \<heavy_comma> \<^bold>h\<^bold>e\<^bold>a\<^bold>p Nothing
+        \<longmapsto> (\<exists>*seg. (R\<heavy_comma> (seg |+ 0) \<tycolon> Pointer \<heavy_comma> \<^bold>h\<^bold>e\<^bold>a\<^bold>p (seg |+ 0) \<R_arr_tail> replicate n zero \<tycolon> Array N)) \<brangle>"
+  for N :: "('x::{zero,field},'b)\<nu>"
+  unfolding \<nu>def op_alloc_def Array_def Heap_Divider_def
+  apply (auto simp add: lrep_exps list_all2_conv_all_nth Let_def same_addr_offset_def nu_exps)
+  apply (rule malloc_split, simp add: heap_assignN_eval)
+  apply (auto simp add: heap_assignN_eval nu_exps) done
+
+
+proc alloc : \<open>R\<heavy_comma> \<^bold>h\<^bold>e\<^bold>a\<^bold>p Nothing\<close> \<longmapsto> \<open>\<exists>*ptr. (R\<heavy_comma> ptr \<tycolon> Pointer\<heavy_comma> \<^bold>h\<^bold>e\<^bold>a\<^bold>p ptr \<R_arr_tail> zero \<tycolon> Ref T)\<close>
+  requires "\<^bold>p\<^bold>a\<^bold>r\<^bold>a\<^bold>m T" and [\<nu>intro]: "\<nu>Zero T zero"
+  have A[simp]: "replicate 1 zero = [zero]" by (simp add: One_nat_def)
+  \<bullet>\<open>1 \<tycolon> \<nat>[size_t]\<close> alloc_array T
+  finish
+
+subsection \<open>Load & Store\<close>
+
+\<nu>overloads \<up> and "\<up>:" and \<Up> and "\<Up>:" and \<down> and "\<down>:" and \<Down> and "\<Down>:"
+
+abbreviation "list_map_at f i l \<equiv> list_update l i (f (l ! i))"
+
+subsubsection \<open>load\<close>
+
+
+lemma op_load[ \<nu>overload "\<up>:" ]:
+  "FieldIndex field_index Y X gt mp \<longrightarrow>
+  \<^bold>p\<^bold>r\<^bold>o\<^bold>c op_load TYPE('y::field) TYPE('x) field_index
+    \<blangle> R\<heavy_comma> addr \<tycolon> Pointer\<heavy_comma> \<^bold>h\<^bold>e\<^bold>a\<^bold>p H \<heavy_asterisk> addr \<R_arr_tail> x \<tycolon> Ref X \<longmapsto> R\<heavy_comma> gt x \<tycolon> Y\<heavy_comma> \<^bold>h\<^bold>e\<^bold>a\<^bold>p H \<heavy_asterisk> addr \<R_arr_tail> x \<tycolon> Ref X\<brangle> "
+  for X :: "('x::field, 'c) \<nu>"
+  unfolding op_load_def Procedure_def FieldIndex_def \<nu>index_def Heap_Divider_def
+  by (cases field_index, cases addr)  (auto simp add: lrep_exps MemAddrState_def nu_exps split: option.split iff: addr_allocated_def)
+
+lemmas [ \<nu>overload "\<up>" ] = op_load[THEN mp, OF FieldIndex_here, simplified]
+
+proc i_load_n[\<nu>overload "\<up>:"]:
+  \<open>a \<tycolon> Pointer\<heavy_comma> i \<tycolon> \<nat>[size_t]\<heavy_comma> \<^bold>h\<^bold>e\<^bold>a\<^bold>p H \<heavy_asterisk> a \<R_arr_tail> xs \<tycolon> Array X\<close> \<longmapsto> \<open>gt (xs ! i) \<tycolon> Y\<heavy_comma> \<^bold>h\<^bold>e\<^bold>a\<^bold>p H \<heavy_asterisk> a \<R_arr_tail> xs \<tycolon> Array X\<close>
+  for Y :: "('y::field, 'd) \<nu>"
+  requires [used]: "\<^bold>p\<^bold>r\<^bold>e\<^bold>m\<^bold>i\<^bold>s\<^bold>e i < length xs" and idx: "FieldIndex field_index Y X gt mp"
+  \<bullet> +\<up>: idx
+  finish
+
+lemmas [ \<nu>overload "\<up>" ] = i_load_n_\<nu>app[THEN mp, THEN mp, OF _ FieldIndex_here, unfolded atomize_imp, simplified]
+
+
+subsubsection \<open>store\<close>
+
+
+lemma op_store[ \<nu>overload "\<down>:" ]:
+  "FieldIndex field_index Y X gt mp \<longrightarrow>
+  \<^bold>p\<^bold>r\<^bold>o\<^bold>c op_store TYPE('y::field) TYPE('x) field_index
+    \<blangle> R\<heavy_comma> addr \<tycolon> Pointer\<heavy_comma> y \<tycolon> Y\<heavy_comma> \<^bold>h\<^bold>e\<^bold>a\<^bold>p addr \<R_arr_tail> x \<tycolon> Ref X \<longmapsto> R \<heavy_comma> \<^bold>h\<^bold>e\<^bold>a\<^bold>p addr \<R_arr_tail> mp (\<lambda>_. y) x \<tycolon> Ref X\<brangle> "
+  for X :: "('x::field, 'c) \<nu>"
+  unfolding op_store_def Procedure_def FieldIndex_def \<nu>index_def Heap_Divider_def Stack_Delimiter_def
+  apply (cases field_index, cases addr)
+  apply (auto simp add: lrep_exps Let_def nu_exps split: option.split iff: addr_allocated_def)
+  subgoal premises prems for x1 x2 x1a x2a aa ofs b x2b H h1 h2 proof -
+    have t1: "\<And>v. (h1 ++ h2)(MemAddress (x1a |+ x2a) \<mapsto> v) = h1 ++ (h2(MemAddress (x1a |+ x2a) \<mapsto> v))"
+      using prems disjoint_rewR by simp
+    have t2: "\<And>v.  dom (h2(MemAddress (x1a |+ x2a) \<mapsto> v)) = dom h2"
+      using prems by auto
+    show ?thesis apply (unfold t1, rule heap_split_id, unfold t2, simp add: prems)
+      using prems by (auto simp add: nu_exps MemAddrState_def)
+  qed done
+
+lemmas [ \<nu>overload "\<down>" ] = op_store[THEN mp, OF FieldIndex_here, simplified]
+
+proc i_store_n[\<nu>overload "\<down>:"]:
+  \<open>R\<heavy_comma> a \<tycolon> Pointer\<heavy_comma> i \<tycolon> \<nat>[size_t]\<heavy_comma> y \<tycolon> Y \<heavy_comma> \<^bold>h\<^bold>e\<^bold>a\<^bold>p a \<R_arr_tail> xs \<tycolon> Array X\<close> \<longmapsto> \<open>R\<heavy_comma> \<^bold>h\<^bold>e\<^bold>a\<^bold>p a \<R_arr_tail> xs[i := mp (\<lambda>_. y) (xs ! i)] \<tycolon> Array X\<close>
+  for Y :: "('y::field, 'd) \<nu>"
+  requires [used]: "\<^bold>p\<^bold>r\<^bold>e\<^bold>m\<^bold>i\<^bold>s\<^bold>e i < length xs" and idx: "FieldIndex field_index Y X gt mp"
+  \<bullet> \<rightarrow> y + y \<down>: idx
+  finish
+
+lemmas [ \<nu>overload "\<down>" ] = i_store_n_\<nu>app[THEN mp, THEN mp, OF _ FieldIndex_here, unfolded atomize_imp, simplified]
+
+
+
+declare Nat.One_nat_def[simp del] Num.add_2_eq_Suc'[simp] split_paired_All[simp]
+
+bundle xx = Nat.One_nat_def[simp del] Num.add_2_eq_Suc'[simp] split_paired_All[simp]
+
+proc times: \<open>R'\<heavy_comma> n \<tycolon> \<nat>['b::len]\<heavy_comma> \<^bold>h\<^bold>e\<^bold>a\<^bold>p H'\<close> \<longmapsto> \<open>\<exists>*x. (R x\<heavy_comma> \<^bold>h\<^bold>e\<^bold>a\<^bold>p H x) \<and>\<^sup>s P x n\<close>
+  requires [unfolded Variant_Cast_def, simp]: "Variant_Cast vars R' H' R H"
+    and \<open>\<^bold>p\<^bold>a\<^bold>r\<^bold>a\<^bold>m P\<close>
+    and [used]: \<open>\<^bold>p\<^bold>r\<^bold>e\<^bold>m\<^bold>i\<^bold>s\<^bold>e P vars 0\<close>
+    and Body: \<open>\<forall>x i. \<^bold>p\<^bold>r\<^bold>e\<^bold>m\<^bold>i\<^bold>s\<^bold>e i < n \<longrightarrow> \<^bold>p\<^bold>r\<^bold>e\<^bold>m\<^bold>i\<^bold>s\<^bold>e P x i \<longrightarrow>
+      \<^bold>p\<^bold>r\<^bold>o\<^bold>c body \<blangle> R x\<heavy_comma> i \<tycolon> \<nat>['b]\<heavy_comma> \<^bold>h\<^bold>e\<^bold>a\<^bold>p H x \<longmapsto> \<exists>*x'. ((R x'\<heavy_comma> \<^bold>h\<^bold>e\<^bold>a\<^bold>p H x') \<and>\<^sup>s P x' (Suc i))\<brangle>\<close>
+  \<bullet> \<rightarrow> n \<open>0 \<tycolon> \<nat>['b]\<close>
+  \<bullet> while var vars i in \<open>R vars\<close>, i heap \<open>H vars\<close> always \<open>i \<le> n \<and> P vars i\<close>
+  \<bullet> \<medium_left_bracket> dup n < \<medium_right_bracket> \<medium_left_bracket> -- i Body i 1 + cast ie \<open>Suc i\<close> \<medium_right_bracket> drop
+  finish
+
+fun fib :: "nat \<Rightarrow> nat" where
+  "fib 0 = 1" | "fib (Suc 0) = 1" | "fib (Suc (Suc n)) = fib n + fib (Suc n)"
+
+(* int fib (int i) { if (i \<le> 1) return 1; else return fib (i-2) + fib (i-1); } *)
+rec_proc Fib: \<open>i \<tycolon> \<nat>[32]\<close> \<longmapsto> \<open>fib i \<tycolon> \<nat>\<^sup>r[32]\<close> var i
+  \<bullet> -- i 1 \<le> if \<medium_left_bracket> \<open>1\<tycolon> \<nat>\<^sup>r[32]\<close> \<medium_right_bracket> \<medium_left_bracket> i 2 - Fib i 1 - Fib + \<medium_right_bracket>
+  \<bullet> cast ie \<open>fib i\<close> affirm by (cases i rule: fib.cases) auto
+  finish
+
+proc Fib2: \<open>i \<tycolon> \<nat>[32]\<close> \<longmapsto> \<open>fib i \<tycolon> \<nat>\<^sup>r[32]\<close>
+  \<bullet> \<rightarrow> i
+  \<bullet> \<open>1\<tycolon> \<nat>\<^sup>r[32]\<close> 1
+  \<bullet> i times var y y' in y, y' \<open>\<lambda>i. y' = fib (Suc i) \<and> y = fib i\<close>
+  \<bullet> \<medium_left_bracket> drop \<rightarrow> y, y' y' y y' + \<medium_right_bracket> drop
+  finish
+
+\<nu>interface hhh = Fib
+\<nu>interface yyy = Fib2
+
+ML_file \<open>codegen/codegen.ML\<close>
+ML_file \<open>codegen/NuSys.ML\<close>
+ML_file \<open>codegen/NuPrime.ML\<close>
+ML_file \<open>codegen/NuLLReps.ML\<close>
+ML_file \<open>codegen/misc.ML\<close>
+ML_file \<open>codegen/Instructions.ML\<close>
+
+\<nu>export_llvm \<open>/tmp/xx.ll\<close>
+
+
+ML \<open>NuCompilation.compile @{theory} (tracing o String.concat)\<close>
+
+
+thm i_store_n_\<nu>app
+thm Fib2_\<nu>app
+thm times_\<nu>compilation
+thm while_\<nu>compilation
+ML \<open>~\<close>
+ML \<open>local open NuCG_NuInstructions in
+infixr 6 <*> <%>
+val (_,a) = NuStd_Base.Fib_gen fake
+val _ = print (tracing o String.concat) a
+end\<close>
+thm i_load_n_\<nu>compilation
+
+ML \<open>local open NuCG_NuInstructions in
+infixr 6 <*> <%>
+val _ = op_call (T_int 51 <%> T_int 52 <%> T_int 53 <%> T_nil) ( T_nil) (pair "hhhh") fake
+val a = op_store (T_int 51) (T_tup (T_int 51 <%> T_int 52)) [1] fake
+val _ = print (tracing o String.concat) a
+end\<close>
+ML \<open>funpow\<close>
+
+ML \<open>local open NuCG_NuInstructions in
+infixr 6 <*> <%>
+val a = (op_constr_tuple (T_int 51 <%> T_int 52 <%> T_int 53)
+  #> op_dup
+  #> op_get_tuple [1] (T_int 51 <%> T_int 52 <%> T_int 53)
+  #> op_set_tuple [1] (T_int 51 <%> T_int 52 <%> T_int 53) (T_int 66)
+  #> op_destr_tuple (T_int 51 <%> T_int 52 <%> T_int 53)) fake
+val _ = print (tracing o String.concat) a
+end\<close>
+ML \<open>local open NuCG in
+infixr 6 <*> <%>
+val c = T_nil <%> T_nil ::[]
+val a = NuCG_NuInstructions.op_do_while (T_int 33 <%> T_ptr <%> T_int 12 <%> T_nil ) (push (V 1)) fake
+val _ = print (tracing o String.concat) a
+end\<close>
+
+term itself
+ML \<open>structure NuCG_Groups = struct
+structure one_class = struct
+fun one _ = 1
+end
+end
+\<close>
+term "num.Bit0"
+term "len_of"
+thm len_bit1
+typ "2 Numeral_Type.bit0"
+typ "Numeral_Type.num1"
+ML \<open>val Type (a,b) = @{typ "(2)"}\<close>
+ML \<open>val Type(a,b) = @{typ "'a itself"}\<close>
+ML \<open>val a0_b = @{term "TYPE('a)"}\<close>
+thm instr_comp_def
+thm alloc_\<nu>compilation
+ML \<open>HashTable.hashMake\<close>
+
+
+
+
+
+
+ML_file \<open>library/compilation.ML\<close>
+ML \<open>String.concatWith\<close>
+ML \<open>NuCompilation.compile (Thm.prop_of @{thm Fib2_\<nu>compilation})\<close>
+ML \<open>String.fields (fn c => c = #".") "A.B.C." |> List.last\<close>
+ML \<open>@{term "TYPE(32)"}\<close>
+thm Fib2_\<nu>compilation
+
+
 
 proc split_array[\<nu>overload split]: \<open>ptr \<tycolon> Pointer\<heavy_comma> n \<tycolon> \<nat>[size_t]\<heavy_comma> \<^bold>h\<^bold>e\<^bold>a\<^bold>p ptr \<R_arr_tail> l \<tycolon> Array T\<close>
   \<longmapsto> \<open>ptr ||+ n \<tycolon> Pointer\<heavy_comma> \<^bold>h\<^bold>e\<^bold>a\<^bold>p ptr \<R_arr_tail> take n l \<tycolon> Array T \<heavy_asterisk> (ptr ||+ n) \<R_arr_tail> drop n l \<tycolon> Array T\<close>
